reworked the properties and shown `Formula As` forms a HA (it's actually just equivalent to `P As`)

Triposes/Language/Properties.lean
@@ -11,26 +11,177 @@ section Algebra
   variable {𝒞 : Type u} [Category.{v, u} 𝒞]
   variable {P : 𝒞ᵒᵖ ⥤ HeytAlg} [T : Tripos P]
 
-  variable {As Bs Cs: 𝒞}
-  variable {f g: As ⟶ Bs}
-  variable (α β : Formula (P := P) As)
-  variable {φ ψ : Formula (P := P) As}
+  variable {As : 𝒞}
 
-  namespace Formula
+  instance : LE (Formula (P := P) As) where
+    le φ ψ := φ.eval ≤ ψ.eval
 
-    def conj_comm : α.conj β = β.conj α := by
-      apply α.ind
-      apply β.ind
-      rintro α β
+  syntax "unfold_quotient_le" : tactic
+  syntax "full_eval" : tactic
+  macro_rules
+    | `(tactic| unfold_quotient_le) =>
+      `(tactic| simp [LE.le, instLEFormula])
+    | `(tactic| full_eval) =>
+      `(tactic| simp [Formula.ι, Formula.app, Formula.impl, Formula.conj, Formula.disj, Formula.all, Formula.any, Formula.eval, Formula'.eval])
+      -- `(tactic| repeat (first | unfold Formula.app | unfold Formula.impl | unfold Formula.conj | unfold Formula.disj | unfold Formula.all | unfold Formula.any))
+
+  instance : Lattice (Formula (P := P) As) where
+  -- instance : HeytingAlgebra (Formula (P := P) As) where
+    le_refl _ := by unfold_quotient_le
+    le_trans _ _ _ := le_trans
+    le_antisymm φ ψ := by
+      induction φ using Quotient.ind
+      induction ψ using Quotient.ind
+      rintro H K
       unfold_quotient
-      apply inf_comm
+      simp [instLEFormula] at H
+      simp [instLEFormula] at K
+      apply_rules [le_antisymm]
+    sup := Formula.disj
+    le_sup_left φ ψ := by
+      induction φ using Quotient.ind
+      induction ψ using Quotient.ind
+      unfold_quotient_le
+      full_eval
+    le_sup_right φ ψ := by
+      induction φ using Quotient.ind
+      induction ψ using Quotient.ind
+      unfold_quotient_le
+      full_eval
+    sup_le φ ψ α := by
+      induction φ using Quotient.ind
+      induction ψ using Quotient.ind
+      rintro H K
+      unfold_quotient_le
+      simp [instLEFormula] at H
+      simp [instLEFormula] at K
+      full_eval
+      tauto
+    inf := Formula.conj
+    inf_le_left φ ψ := by
+      induction φ using Quotient.ind
+      induction ψ using Quotient.ind
+      unfold_quotient_le
+      full_eval
+    inf_le_right φ ψ := by
+      induction φ using Quotient.ind
+      induction ψ using Quotient.ind
+      unfold_quotient_le
+      full_eval
+    le_inf φ ψ α := by
+      induction φ using Quotient.ind
+      induction ψ using Quotient.ind
+      induction α using Quotient.ind
+      rintro H K
+      unfold_quotient_le
+      simp [instLEFormula] at H
+      simp [instLEFormula] at K
+      full_eval
+      tauto
 
-    def disj_comm : α.disj β = β.disj α := by
-      apply α.ind
-      apply β.ind
-      rintro α β
+  instance : HeytingAlgebra (Formula (P := P) As) where
+    himp := Formula.impl
+    le_himp_iff φ ψ α := by
+      apply φ.ind; apply ψ.ind; apply α.ind; rintro φ ψ α
+      constructor
+      · rintro H
+        unfold LE.le Preorder.toLE PartialOrder.toPreorder SemilatticeSup.toPartialOrder
+        unfold Lattice.toSemilatticeSup instLatticeFormula instLEFormula Formula.eval; simp
+        conv =>
+          enter [1]
+          tactic =>
+            unfold min SemilatticeInf.toMin SemilatticeInf.inf Lattice.toSemilatticeInf Formula.conj; simp
+        conv => lhs; unfold Formula'.eval
+        unfold LE.le Preorder.toLE PartialOrder.toPreorder SemilatticeSup.toPartialOrder at H
+        unfold Lattice.toSemilatticeSup instLatticeFormula instLEFormula at H
+        unfold Formula.eval Formula.impl at H; simp at H
+        conv at H => rhs; unfold Formula'.eval
+        apply_rules [le_himp_iff.mp]
+      · rintro H
+        unfold LE.le Preorder.toLE PartialOrder.toPreorder SemilatticeSup.toPartialOrder
+        unfold Lattice.toSemilatticeSup instLatticeFormula instLEFormula
+        unfold Formula.eval Formula.impl; simp
+        conv => rhs; unfold Formula'.eval
+        unfold LE.le Preorder.toLE PartialOrder.toPreorder SemilatticeSup.toPartialOrder at H
+        unfold Lattice.toSemilatticeSup instLatticeFormula instLEFormula at H
+        unfold Formula.eval at H; simp at H
+        conv at H =>
+          enter [1]
+          tactic =>
+            unfold min SemilatticeInf.toMin SemilatticeInf.inf Lattice.toSemilatticeInf Formula.conj; simp
+        conv at H => lhs; unfold Formula'.eval
+        apply_rules [le_himp_iff.mpr]
+    top := Formula.tru
+    le_top φ := le_top
+    bot := Formula.fal
+    bot_le φ := bot_le
+    compl x := x.impl Formula.fal
+    himp_bot _ := rfl
+
+  section Formula
+    variable (α β γ : Formula (P := P) As)
+
+    def conj_top_eq : α.conj ⊤ = α := inf_top_eq α
+    def top_conj_eq : Formula.tru.conj α = α := top_inf_eq α
+    def conj_comm : α.conj β = β.conj α := inf_comm α β
+    def conj_idem : α.conj α = α := inf_idem α
+    def conj_assoc : (α.conj β).conj γ = α.conj (β.conj γ) := inf_assoc α β γ
+    variable {β γ}
+    def conj_le_conj_left : β ≤ γ → α.conj β ≤ α.conj γ := inf_le_inf_left α
+    def conj_le_conj_right : β ≤ γ → β.conj α ≤ γ.conj α := inf_le_inf_right α
+    variable {α}
+    def conj_le_left : α.conj β ≤ α := inf_le_left
+    def conj_le_right : α.conj β ≤ β := inf_le_right
+    def le_conj : α ≤ β → α ≤ γ → α ≤ β.conj γ := le_inf
+    def conj_eq_left : α.conj β = α ↔ α ≤ β := inf_eq_left
+    def conj_eq_right : α.conj β = β ↔ β ≤ α := inf_eq_right
+    def left_eq_conj : α = α.conj β ↔ α ≤ β := left_eq_inf
+    def right_eq_conj : β = α.conj β ↔ β ≤ α := right_eq_inf
+
+    variable (α β γ)
+    def disj_comm : α.disj β = β.disj α := sup_comm α β
+    def disj_idem : α.disj α = α := sup_idem α
+    def disj_assoc : (α.disj β).disj γ = α.disj (β.disj γ) := sup_assoc α β γ
+
+    def impl_conj_distrib : α.impl (β.conj γ) = (α.impl β).conj (α.impl γ) := himp_inf_distrib α β γ
+    variable {α β} in
+    def impl_eq_top_iff : α.impl β = ⊤ ↔ α ≤ β := himp_eq_top_iff
+    variable {a} in
+    def impl_self : α.impl α = ⊤ := himp_self
+
+    lemma tru_eq_tru : Formula.tru (As := As) = q (P := P) Formula'.tru := by unfold_quotient
+
+    variable {α β} in
+    theorem conj_eq_top_iff : α.conj β = Formula.tru ↔ α = Formula.tru ∧ β = Formula.tru := by
+      induction α using Quotient.ind
+      induction β using Quotient.ind
+      constructor
+      · rintro H
+        replace H := Quotient.eq.mp H
+        simp [Formula'.eval] at H
+        simp
+        replace ⟨H, K⟩ := H
+        constructor
+        all_goals unfold_quotient; assumption
+      · rintro ⟨H, K⟩
+        rw [H, K]
+        unfold_quotient; full_eval
+
+    lemma iota_eval : Formula.ι (α.eval) = α := by
+      induction α using Quotient.ind
       unfold_quotient
-      apply sup_comm
+      full_eval
+
+    variable {α β}
+    def biimpl_eq_top_iff : (α.impl β).conj (β.impl α) = ⊤ ↔ α = β := by
+      constructor
+      · rintro H
+        replace ⟨H, K⟩ := conj_eq_top_iff.mp H
+        replace H := impl_eq_top_iff.mp H
+        replace K := impl_eq_top_iff.mp K
+        exact le_antisymm H K
+      · rintro rfl
+        rw [impl_self, conj_idem]
 
   end Formula
 end Algebra
@@ -42,98 +193,198 @@ section Map
 
   variable {As Bs Cs: 𝒞}
   variable {f : As ⟶ Bs} {g : Bs ⟶ Cs}
-  variable {γ : Formula (P := P) Cs}
+  variable {α α' : Formula (P := P) As} {β β' : Formula (P := P) Bs} {γ : Formula (P := P) Cs}
 
-  -- @[simp]
-  -- theorem map_id {X : 𝒞} {x : P₀ (P := P) X} : Formula.app x (𝟙 X) = x := by
-  --   unfold_quotient
-  --   aesop_cat
-
-  theorem map_comp_app : γ.app (f ≫ g) = (γ.app g).app f := by
-    apply γ.ind
-    rintro γ
+  @[simp]
+  theorem map_id : Formula.app α (𝟙 As) = α := by
+    induction α using Quotient.ind
     unfold_quotient
+    full_eval
     aesop_cat
 
-  instance : LE (Formula (P := P) As) := by
-    constructor
-    rintro φ ψ
-    exact φ.eval ≤ ψ.eval
+  theorem map_comp_app : γ.app (f ≫ g) = (γ.app g).app f := by
+    induction γ using Quotient.ind
+    unfold_quotient
+    simp [Formula'.eval]
+    aesop_cat
 
-  -- macro_rules
-  --   | `(tactic| unfold_quotient) =>
-  --     `(tactic| apply Quot.sound; unfold Formula_Eq; unfold Formula'.eval; simp)
-  syntax "unfold_quotient_le" : tactic
-  syntax "full_eval" : tactic
-  macro_rules
-    | `(tactic| unfold_quotient_le) =>
-      `(tactic| unfold LE.le; unfold instLEFormula; simp)
-    | `(tactic| full_eval) =>
-      `(tactic| repeat (first | unfold Formula.app | unfold Formula.impl | unfold Formula.conj | unfold Formula.disj | unfold Formula.all | unfold Formula.any))
+  theorem map_top_eq_top : Formula.app (P := P) ⊤ f = ⊤ := by
+    unfold_quotient
+    full_eval
+
+  theorem map_conj : (β.conj β').app f = (β.app f).conj (β'.app f) := by
+    induction β using Quotient.ind
+    induction β' using Quotient.ind
+    unfold_quotient
+    full_eval
+
+  theorem map_disj : (β.disj β').app f = (β.app f).disj (β'.app f) := by
+    induction β using Quotient.ind
+    induction β' using Quotient.ind
+    unfold_quotient
+    full_eval
+
+  theorem map_impl : (β.impl β').app f = (β.app f).impl (β'.app f) := by
+    induction β using Quotient.ind
+    induction β' using Quotient.ind
+    unfold_quotient
+    full_eval
+
+  variable (f) (β) in
+  theorem weakening : β.app f ≤ α → β = ⊤ → α = ⊤ := by
+    induction α using Quotient.ind
+    induction β using Quotient.ind
+    rintro le isTop
+    rw [isTop] at le
+    apply eq_top_iff.mpr
+    trans Formula.app ⊤ f
+    · apply le_of_eq
+      unfold_quotient
+      full_eval
+    · exact le
+
+  theorem map_monotone : β ≤ β' → β.app f ≤ β'.app f := by
+    induction β using Quotient.ind
+    induction β' using Quotient.ind
+    intro H
+    exact P₁.map_mono H
 
 end Map
+
+section FPCat
+  universe u v
+  variable {𝒞 : Type u} [Category.{v, u} 𝒞] [fp : ChosenFiniteProducts 𝒞]
+  variable {P : 𝒞ᵒᵖ ⥤ HeytAlg} [T : Tripos P]
+
+  variable {X Y Z : 𝒞}
+  open ChosenFiniteProducts
+
+  theorem lift_diag {f : X ⟶ Y} : lift f f = f ≫ diag := by unfold diag; aesop_cat
+  theorem lift_snd_fst : lift (fp.snd X Y) (fp.fst X Y) = twist := by unfold twist; aesop_cat
+  theorem comp_lift_left {f : X ⟶ Y} {g : Y ⟶ Z} : lift (f ≫ g) f = f ≫ lift g (𝟙 _) := by aesop_cat
+  theorem comp_lift_right {f : X ⟶ Y} {g : Y ⟶ Z} : lift f (f ≫ g) = f ≫ lift (𝟙 _) g := by aesop_cat
+  theorem lift_comp_fst_comp_snd {f : X ⟶ Y ⊗ Z} : lift (f ≫ fp.fst _ _) (f ≫ fp.snd _ _) = f := by aesop_cat
+  theorem diag_fst : diag ≫ fp.fst _ _ = 𝟙 X := by unfold diag; aesop_cat
+  theorem diag_snd : diag ≫ fp.snd _ _ = 𝟙 X := by unfold diag; aesop_cat
+
+  syntax "simp_proj" : tactic
+  syntax "simp_proj_only" : tactic
+  macro_rules
+    | `(tactic| simp_proj_only) =>
+      `(tactic| simp only
+        [comp_lift, lift_fst, lift_snd, lift_diag, lift_snd_fst, lift_fst_snd, lift_comp_fst_comp_snd,
+        ←Category.assoc, Category.id_comp, Category.comp_id, ←P₁.map_comp_app, P₁.map_inf, P₁.map_sup, P₁.map_himp])
+    | `(tactic| simp_proj) =>
+      `(tactic| simp
+        [comp_lift, lift_fst, lift_snd, lift_diag, lift_snd_fst, lift_fst_snd, lift_comp_fst_comp_snd, diag_fst, diag_snd, ←Category.assoc, Category.id_comp, Category.comp_id, ←map_comp_app, map_conj, map_disj, map_impl])
+
+end FPCat
+
 namespace Any
   universe u v
   variable {𝒞 : Type u} [Category.{v, u} 𝒞]
   variable {P : 𝒞ᵒᵖ ⥤ HeytAlg} [T : Tripos P]
 
-  variable {X Y Z As Bs Cs: 𝒞}
+  variable {X Y Z As Bs Cs : 𝒞}
   variable {f : As ⟶ Bs} {g : Bs ⟶ Cs}
   variable {x : P₀ (P := P) X} {y : P₀ (P := P) Y} {z : P₀ (P := P) Z}
   variable {φ : Formula (P := P) X} {ψ : Formula (P := P) Y}
-  variable {α : Formula (P := P) As} {β : Formula (P := P) Bs} {γ : Formula (P := P) Cs}
+  variable {α α' : Formula (P := P) As} {β : Formula (P := P) Bs} {γ : Formula (P := P) Cs}
+
+  lemma adj : (α ≤ β.app f) ↔ (Formula.any f α ≤ β) := by
+    induction α using Quotient.ind
+    induction β using Quotient.ind
+    constructor
+    · rintro H
+      unfold_quotient_le
+      exact (T.𝔼 _).adj.mp H
+    · rintro H
+      unfold_quotient_le
+      exact (T.𝔼 _).adj.mpr H
 
   lemma unit : α ≤ Formula.app (Formula.any f α) f := by
+    induction α using Quotient.ind
     unfold_quotient_le
-    apply α.ind
-    rintro α
     full_eval
-    simp
-    apply (T.𝔼 _).unit
+    exact (T.𝔼 _).unit
 
   lemma counit : Formula.any f (Formula.app β f) ≤ β := by
-    apply β.ind
-    intros
+    induction β using Quotient.ind
     unfold_quotient_le
     full_eval
-    simp
-    apply (T.𝔼 _).counit
+    exact (T.𝔼 _).counit
 
   lemma id_adj_id : Formula.any (𝟙 _) α = α := by
-    apply α.ind
-    rintro α
+    induction α using Quotient.ind
+    unfold_quotient
     full_eval
-    simp
-    apply Quot.sound
-    unfold Formula_Eq
-    conv => lhs; unfold Formula'.eval
     rw [(T.𝔼 _).id_adj_id]
     simp
 
   lemma frob_left : Formula.any f (α.conj (β.app f)) = (Formula.any f α).conj β := by
-    apply α.ind
-    apply β.ind
-    rintro α β
+    induction α using Quotient.ind
+    induction β using Quotient.ind
     unfold_quotient
-    conv => lhs; unfold Formula'.eval; enter [2, 2]; unfold Formula'.eval
-    conv => enter [2, 1]; unfold Formula'.eval
+    full_eval
     apply (T.𝔼 _).frob_left
 
   lemma frob_right : Formula.any f ((β.app f).conj α) = β.conj (Formula.any f α) := by
-    rw [Formula.conj_comm, Formula.conj_comm β]
+    rw [conj_comm, conj_comm β]
     exact frob_left
+
+  lemma monotone : α ≤ α' → Formula.any f α ≤ Formula.any f α' := by
+    induction α using Quotient.ind
+    induction α' using Quotient.ind
+    rintro H
+    exact (T.𝔼 _).map.monotone H
 
   section BC
     variable {X Y Z W : 𝒞} {f : X ⟶ Y} {g : X ⟶ Z} {h : Y ⟶ W} {k : Z ⟶ W}
 
     def BeckChevalley : IsPullback f g h k → ∀ {z : Formula (P := P) Z}, Formula.any f (z.app g) = (Formula.any k z).app h := by
       rintro isPB z
-      apply z.ind
-      intros
+      induction z using Quotient.ind
       unfold_quotient
-      unfold Formula'.eval
+      full_eval
       apply T.𝔼_BeckChevalley isPB
   end BC
+
+  theorem comp_app
+    : Formula.any g (Formula.any f α) = Formula.any (f ≫ g) α := by
+      apply le_antisymm
+      · repeat apply adj.mp
+        rw [←map_comp_app]
+        have isPB : IsPullback (𝟙 _) (𝟙 _) (f ≫ g) (f ≫ g) := by sorry
+        simp [←BeckChevalley isPB, id_adj_id]
+      · apply adj.mp
+        rw [map_comp_app]
+        have isPB : IsPullback (𝟙 _) (𝟙 _) (g) (g) := by sorry
+        have isPB' : IsPullback (𝟙 _) (𝟙 _) (f) (f) := by sorry
+        simp [←BeckChevalley isPB, ←BeckChevalley isPB', id_adj_id]
+
+  variable (f) in
+  theorem iso_app {φ : IsIso f} : Formula.any g β = Formula.any (f ≫ g) (β.app f) := by
+    have isPB : IsPullback (f ≫ g) (f) (𝟙 _) (g) := by
+      apply IsPullback.of_iso (IsPullback.id_vert g)
+      case e₁ => exact {
+        hom := inv f
+        inv := f
+      }
+      case e₂ => exact Iso.refl Cs
+      case e₃ => exact Iso.refl Bs
+      case e₄ => exact Iso.refl Cs
+      all_goals aesop_cat
+    rw [BeckChevalley isPB]
+    simp
+
+  open ChosenFiniteProducts
+  theorem comm_app [fp : ChosenFiniteProducts 𝒞] {φ : Formula (P := P) ((X ⊗ Y) ⊗ Z)}
+    : Formula.any (fp.fst X Y) (Formula.any (fp.fst (X ⊗ Y) Z) φ) = Formula.any (fp.fst X Z) (Formula.any (fp.fst (X ⊗ Z) Y) (φ.app (x : X, z : Z, y : Y ⊢ₑ ⟨⟨x, y⟩, z⟩))) := by
+      repeat rw [comp_app]
+      rw [iso_app (x : X, z : Z, y : Y ⊢ₑ ⟨⟨x, y⟩, z⟩)]
+      · simp_proj
+      · use x : X, y : Y, z : Z ⊢ₑ ⟨⟨x, z⟩, y⟩
+        aesop_cat
 end Any
 
 namespace All
@@ -145,62 +396,71 @@ namespace All
   variable {f : As ⟶ Bs} {g : Bs ⟶ Cs}
   variable {x : P₀ (P := P) X} {y : P₀ (P := P) Y} {z : P₀ (P := P) Z}
   variable {φ : Formula (P := P) X} {ψ : Formula (P := P) Y}
-  variable {α : Formula (P := P) As} {β : Formula (P := P) Bs} {γ : Formula (P := P) Cs}
+  variable {α α' : Formula (P := P) As} {β : Formula (P := P) Bs} {γ : Formula (P := P) Cs}
+
+  lemma adj : (β.app f ≤ α) ↔ (β ≤ Formula.all f α) := by
+    induction α using Quotient.ind
+    induction β using Quotient.ind
+    constructor
+    · rintro H
+      unfold_quotient_le
+      full_eval
+      exact (T.𝔸 _).adj.mp H
+    · rintro H
+      unfold_quotient_le
+      full_eval
+      exact (T.𝔸 _).adj.mpr H
 
   lemma unit : β ≤ Formula.all f (Formula.app β f) := by
+    induction β using Quotient.ind
     unfold_quotient_le
-    apply β.ind
-    rintro β
     full_eval
-    simp
-    apply (T.𝔸 _).unit
+    exact (T.𝔸 _).unit
 
   lemma counit : Formula.app (Formula.all f α) f ≤ α := by
-    apply α.ind
-    rintro α
+    induction α using Quotient.ind
     unfold_quotient_le
     full_eval
-    simp
-    apply (T.𝔸 _).counit
+    exact (T.𝔸 _).counit
 
   lemma id_adj_id : Formula.all (𝟙 _) α = α := by
-    apply α.ind
-    rintro α
+    induction α using Quotient.ind
+    unfold_quotient
     full_eval
-    simp
-    apply Quot.sound
-    unfold Formula_Eq
-    conv => lhs; unfold Formula'.eval
     rw [(T.𝔸 _).id_adj_id]
     simp
 
-  lemma top_eq_top : Formula.all f Formula.tru = Formula.tru (T := T) := by
+  -- lemma top_eq_top : (y : Y ⊢ₕ ∀ x : X , ⊤) = (y : Y ⊢ₕ ⊤ : Formula _ (T := T)) := by
+  lemma top_eq_top : Formula.all (T := T) f ⊤ = ⊤ := by
     unfold_quotient
-    unfold Formula'.eval
-    apply (T.𝔸 _).top_eq_top
+    full_eval
+    exact (T.𝔸 _).top_eq_top
 
-  -- lemma frob_left : Formula.all f (α.disj (β.app f)) = (Formula.all f α).disj β := by
-  --   apply α.ind
-  --   apply β.ind
-  --   rintro α β
-  --   unfold_quotient
-  --   conv => lhs; unfold Formula'.eval; enter [2, 2]; unfold Formula'.eval
-  --   conv => enter [2, 1]; unfold Formula'.eval
-  --   apply (T.𝔸 _).frob_left
+  variable (f) in
+  lemma eq_top_iff_forall_eq_top : α = ⊤ ↔ (Formula.all f α) = ⊤ := by
+    constructor
+    · rintro rfl
+      exact top_eq_top
+    · rintro H
+      apply eq_top_iff.mpr
+      rw [←map_top_eq_top (f := f)]
+      apply All.adj.mpr
+      rw [H]
 
-  -- lemma frob_right : Formula.all f ((β.app f).disj α) = β.disj (Formula.all f α) := by
-  --   rw [Formula.disj_comm, Formula.disj_comm β]
-  --   exact frob_left
+  lemma monotone : α ≤ α' → Formula.all f α ≤ Formula.all f α' := by
+    induction α using Quotient.ind
+    induction α' using Quotient.ind
+    rintro H
+    exact (T.𝔸 _).map.monotone H
 
   section BC
     variable {X Y Z W : 𝒞} {f : X ⟶ Y} {g : X ⟶ Z} {h : Y ⟶ W} {k : Z ⟶ W}
 
     def BeckChevalley : IsPullback f g h k → ∀ {z : Formula (P := P) Z}, Formula.all f (z.app g) = (Formula.all k z).app h := by
       rintro isPB z
-      apply z.ind
-      intros
+      induction z using Quotient.ind
       unfold_quotient
-      unfold Formula'.eval
+      full_eval
       apply T.𝔸_BeckChevalley isPB
   end BC
 end All
@@ -216,13 +476,11 @@ section Adjoints
   variable {φ : Formula (P := P) X} {ψ : Formula (P := P) Y}
   variable {α : Formula (P := P) As} {β : Formula (P := P) Bs} {γ : Formula (P := P) Cs}
 
-  lemma frobenius : Formula.all f (α.impl (Formula.app β f)) = (Formula.any f α).impl β := by
-    apply α.ind
-    apply β.ind
-    intros
+  lemma frobenius : Formula.all f (α ⇨ (Formula.app β f)) = (Formula.any f α) ⇨ β := by
+    induction α using Quotient.ind
+    induction β using Quotient.ind
     unfold_quotient
-    conv => lhs; unfold Formula'.eval; enter [2, 2]; unfold Formula'.eval
-    conv => enter [2, 1]; unfold Formula'.eval
+    full_eval
     apply T.frobenius
 
 end Adjoints
